\documentclass{article}
\usepackage{epsfig}
\pagestyle{empty}
\begin{document}
$\epsilon$
\pagebreak

\begin{equation} \frac {\partial} {\partial t} \left[\begin{array}{c} \rho \\ \rho u \\ e \end{array}\right] + \frac {\partial} {\partial x} \left[\begin{array}{c} \rho u \\ \rho u^2 + p \\ (e+p) u\end{array}\right] = \left[\begin{array}{c} 0 \\ -\rho g \\ -\rho u g \end{array}\right] \end{equation}
\pagebreak

\begin{equation} e = \frac {p} {\gamma-1} + \frac{1}{2} \rho u^2 \end{equation}
\pagebreak

$\gamma$
\pagebreak

\begin{align} {\bf U}^{\left(i\right)} &= {\bf u}_n + \delta t \sum_{j=1}^{i-1} A_{ij} \dot{\bf U}^{\left(j\right)}\ {\rm (Stage\ values)},\\ {\bf u}_{n+1} &= {\bf u}_n + \delta t \sum_{i=1}^{n} b_i \dot{\bf U}^{\left(i\right)}\ {\rm (Step\ completion)}, \end{align}
\pagebreak

${\bf u}_n$
\pagebreak

${\bf u}_{n+1}$
\pagebreak

$A_{ij}$
\pagebreak

$b_i$
\pagebreak

$y-\tilde{y}$
\pagebreak

$y-\epsilon$
\pagebreak

\begin{equation} {\bf F}\left({\bf u}\right) = \left[\begin{array}{c} \rho u \\ \rho u^2 + p \\ (e+p) u \end{array}\right] \end{equation}
\pagebreak

\begin{equation} {\bf F}_F\left({\bf u}\right) = A_f\left({\bf u}\right){\bf u} \end{equation}
\pagebreak

$A_f\left({\bf u}\right) $
\pagebreak

$A_f$
\pagebreak

\begin{equation} {\bf f}_{j+1/2} = \frac{1}{2}\left[ {\bf f}_{j+1/2}^L + {\bf f}_{j+1/2}^R - \left| A\left({\bf u}_{j+1/2}^L,{\bf u}_{j+1/2}^R\right) \right| \left( {\bf u}_{j+1/2}^R - {\bf u}_{j+1/2}^L \right)\right] \end{equation}
\pagebreak

\begin{align} \alpha_{j+1/2}^{k,L} &= \sum_{k=1}^3 {\bf l}_{j+1/2}^k \cdot {\bf f}_{j+1/2}^{k,L}, \\ \alpha_{j+1/2}^{k,R} &= \sum_{k=1}^3 {\bf l}_{j+1/2}^k \cdot {\bf f}_{j+1/2}^{k,R}, \\ v_{j+1/2}^{k,L} &= \sum_{k=1}^3 {\bf l}_{j+1/2}^k \cdot {\bf u}_{j+1/2}^{k,L}, \\ v_{j+1/2}^{k,R} &= \sum_{k=1}^3 {\bf l}_{j+1/2}^k \cdot {\bf u}_{j+1/2}^{k,R}, \\ \alpha_{j+1/2}^k &= \left\{ \begin{array}{cc} \alpha_{j+1/2}^{k,L} & {\rm if}\ \lambda_{j,j+1/2,j+1} > 0 \\ \alpha_{j+1/2}^{k,R} & {\rm if}\ \lambda_{j,j+1/2,j+1} < 0 \\ \frac{1}{2}\left[ \alpha_{j+1/2}^{k,L} + \alpha_{j+1/2}^{k,R} - \left(\max_{\left[j,j+1\right]} \lambda\right) \left( v_{j+1/2}^{k,R} - v_{j+1/2}^{k,L} \right) \right] & {\rm otherwise} \end{array}\right., \\ {\bf f}_{j+1/2} &= \sum_{k=1}^3 \alpha_{j+1/2}^k {\bf r}_{j+1/2}^k \end{align}
\pagebreak

${\bf l}$
\pagebreak

${\bf r}$
\pagebreak

$\lambda$
\pagebreak

\begin{align} \alpha_{j+1/2}^{k,L} &= \sum_{k=1}^3 {\bf l}_{j+1/2}^k \cdot {\bf f}_{j+1/2}^{k,L}, \\ \alpha_{j+1/2}^{k,R} &= \sum_{k=1}^3 {\bf l}_{j+1/2}^k \cdot {\bf f}_{j+1/2}^{k,R}, \\ v_{j+1/2}^{k,L} &= \sum_{k=1}^3 {\bf l}_{j+1/2}^k \cdot {\bf u}_{j+1/2}^{k,L}, \\ v_{j+1/2}^{k,R} &= \sum_{k=1}^3 {\bf l}_{j+1/2}^k \cdot {\bf u}_{j+1/2}^{k,R}, \\ \alpha_{j+1/2}^k &= \frac{1}{2}\left[ \alpha_{j+1/2}^{k,L} + \alpha_{j+1/2}^{k,R} - \left(\max_{\left[j,j+1\right]} \lambda\right) \left( v_{j+1/2}^{k,R} - v_{j+1/2}^{k,L} \right) \right], \\ {\bf f}_{j+1/2} &= \sum_{k=1}^3 \alpha_{j+1/2}^k {\bf r}_{j+1/2}^k \end{align}
\pagebreak

$ u\pm a$
\pagebreak

\end{document}
